proof/ktcore.v
@@ -3,7 +3,7 @@ From New.proof.github_com.sanjit_bhat.pav.ktcore_proof Require Export
 
 Module Import ktcore.
   Export agree.ktcore base.ktcore blame.ktcore evidence.ktcore key_map.ktcore
-    ktcore.ktcore serde.ktcore sigpred.ktcore staged_keys.ktcore.
+    ktcore.ktcore serde.ktcore staged_keys.ktcore.
 End ktcore.
 
 Export sigpred.sigpred.
